proof/agp32_EX_CorrectScript.sml
@@ -95,27 +95,10 @@ val carry_flag_unchanged_by_func_tac =
 
 (* lemmas *)
 (** lemmas copied from the hardware/ag32 repo **)
-Theorem ALU_correct_carry_lem:
-  !(w:33 word). word_bit 32 w <=> n2w (dimword(:32)) <=+ w
-Proof
-  simp [] >> BBLAST_PROVE_TAC
-QED
 
-Theorem ALU_correct_v2w_carry33_lem:
-  !b. v2w [b] = if b then (1w:33 word) else 0w
-Proof
-  Cases >> EVAL_TAC
-QED
 (** copy end **)
                                               
-Theorem w2n_add_MOD_itself:
-  !(w1:word32) (w2:word32).
-    w2n w1 + w2n w2 = (w2n w1 + w2n w2) MOD 8589934592
-Proof
-  rw [] >>
-  `(w2n w1 < 4294967296) /\ (w2n w2 < 4294967296)` by METIS_TAC [w2n_lt,dimword_32] >>
-  fs []
-QED
+
 
 (* carry_flag between ISA and circuit states *)
 Theorem agp32_Rel_ag32_carry_flag_correct:
@@ -302,7 +285,27 @@ Proof
     fs [EX_ALU_update_def]) >>
   cheat
 QED
-*)
+ *)
+
+
+(** lemmas about words for ALU **)
+Theorem ALU_correct_carry_lem:
+  !(w:33 word). word_bit 32 w <=> n2w (dimword(:32)) <=+ w
+Proof
+  simp [] >> BBLAST_PROVE_TAC
+QED
+
+Theorem ALU_correct_v2w_carry33_lem:
+  !b. v2w [b] = if b then (1w:33 word) else 0w
+Proof
+  Cases >> EVAL_TAC
+QED
+
+Theorem ALU_correct_v2w_carry32_lem:
+  !b. v2w [b] = if b then (1w:32 word) else 0w
+Proof
+  Cases >> EVAL_TAC
+QED
 
 
 (** EX_PC_sel **)
@@ -645,6 +648,166 @@ Proof
   fs [Rel_def,EX_Rel_def]
 QED
 
+(** EX_imm_updated **)
+(** when opc is not 14w **)
+Theorem agp32_Rel_ag32_EX_imm_updated_correct_not_LoadUpperConstant:
+  !fext fbits a t I.
+    is_sch_execute I (agp32 fext fbits) a ==>
+    is_sch_disable I (agp32 fext fbits) ==>
+    Rel I (fext t) (agp32 fext fbits (t-1)) (agp32 fext fbits t) a t ==>
+    I (3,SUC t) <> NONE ==>
+    (agp32 fext fbits (SUC t)).EX.EX_opc <> 14w ==>
+    (agp32 fext fbits (SUC t)).EX.EX_imm_updated = imm (FUNPOW Next (THE (I (3,SUC t)) − 1) a)
+Proof
+  rw [] >> Q.ABBREV_TAC `s = agp32 fext fbits t` >>
+  Q.ABBREV_TAC `s' = procs [agp32_next_state;WB_pipeline;MEM_pipeline;EX_pipeline;
+                            REG_write;ID_pipeline;IF_PC_update;Acc_compute] (fext t) s s` >>
+  Q.ABBREV_TAC `s'' = procs [IF_instr_update;ID_opc_func_update;ID_imm_update;ID_data_update;
+                             ID_data_check_update;EX_ctrl_update] (fext (SUC t)) s' s'` >>
+  `(agp32 fext fbits (SUC t)).EX.EX_imm_updated =
+  (EX_ALU_input_imm_update (fext (SUC t)) s' s'').EX.EX_imm_updated`
+    by fs [agp32_EX_imm_updated_updated_by_EX_ALU_input_imm_update] >>
+  `s'.EX.EX_opc = (agp32 fext fbits (SUC t)).EX.EX_opc`
+    by fs [agp32_same_EX_pipeline_items_after_EX_pipeline] >>
+  `s''.EX.EX_imm = (agp32 fext fbits (SUC t)).EX.EX_imm`
+    by METIS_TAC [Abbr `s`,Abbr `s'`,Abbr `s''`,agp32_same_items_after_EX_ctrl_update] >>
+  fs [EX_ALU_input_imm_update_def,MUX_21_def] >>
+  METIS_TAC [agp32_Rel_ag32_EX_imm_correct]
+QED
+
+(** when opc is 14w **)
+Theorem agp32_Rel_ag32_EX_imm_updated_correct_LoadUpperConstant:
+  !fext fbits a t I.
+    is_sch_execute I (agp32 fext fbits) a ==>
+    is_sch_disable I (agp32 fext fbits) ==>
+    Rel I (fext t) (agp32 fext fbits (t-1)) (agp32 fext fbits t) a t ==>
+    I (3,SUC t) <> NONE ==>
+    (agp32 fext fbits (SUC t)).EX.EX_opc = 14w ==>
+    (agp32 fext fbits (SUC t)).EX.EX_imm_updated =
+    (8 >< 0) (imm (FUNPOW Next (THE (I (3,SUC t)) − 1) a)) @@
+             (22 >< 0) (dataW (FUNPOW Next (THE (I (3,SUC t)) − 1) a))
+Proof
+  rw [] >> Q.ABBREV_TAC `s = agp32 fext fbits t` >>
+  Q.ABBREV_TAC `s' = procs [agp32_next_state;WB_pipeline;MEM_pipeline;EX_pipeline;
+                            REG_write;ID_pipeline;IF_PC_update;Acc_compute] (fext t) s s` >>
+  Q.ABBREV_TAC `s'' = procs [IF_instr_update;ID_opc_func_update;ID_imm_update;ID_data_update;
+                             ID_data_check_update;EX_ctrl_update] (fext (SUC t)) s' s'` >>
+  `(agp32 fext fbits (SUC t)).EX.EX_imm_updated =
+  (EX_ALU_input_imm_update (fext (SUC t)) s' s'').EX.EX_imm_updated`
+    by fs [agp32_EX_imm_updated_updated_by_EX_ALU_input_imm_update] >>
+  `s'.EX.EX_opc = (agp32 fext fbits (SUC t)).EX.EX_opc`
+    by fs [agp32_same_EX_pipeline_items_after_EX_pipeline] >>
+  `(s''.EX.EX_imm = (agp32 fext fbits (SUC t)).EX.EX_imm) /\
+  (s''.EX.EX_dataW = (agp32 fext fbits (SUC t)).EX.EX_dataW)`
+    by METIS_TAC [Abbr `s`,Abbr `s'`,Abbr `s''`,agp32_same_items_after_EX_ctrl_update] >>
+  fs [EX_ALU_input_imm_update_def,MUX_21_def] >>
+  METIS_TAC [agp32_Rel_ag32_EX_imm_correct,agp32_Rel_ag32_EX_dataW_correct]
+QED
+
+(** EX_ALU_input **)
+Theorem agp32_Rel_ag32_EX_ALU_input1_correct:
+  !fext fbits a t I.
+    is_sch_execute I (agp32 fext fbits) a ==>
+    is_sch_disable I (agp32 fext fbits) ==>
+    Rel I (fext t) (agp32 fext fbits (t-1)) (agp32 fext fbits t) a t ==>
+    I (3,SUC t) <> NONE ==>
+    (agp32 fext fbits (SUC t)).EX.EX_ALU_input1 = ALU_input1 (FUNPOW Next (THE (I (3,SUC t)) − 1) a)
+Proof
+  rw [] >> Q.ABBREV_TAC `s = agp32 fext fbits t` >>
+  Q.ABBREV_TAC `s' = procs [agp32_next_state;WB_pipeline;MEM_pipeline;EX_pipeline;
+                            REG_write;ID_pipeline;IF_PC_update;Acc_compute] (fext t) s s` >>
+  Q.ABBREV_TAC `s'' = procs [IF_instr_update;ID_opc_func_update;ID_imm_update;ID_data_update;
+                             ID_data_check_update;EX_ctrl_update] (fext (SUC t)) s' s'` >>
+  `(agp32 fext fbits (SUC t)).EX.EX_ALU_input1 =
+  (EX_ALU_input_imm_update (fext (SUC t)) s' s'').EX.EX_ALU_input1`
+    by fs [agp32_EX_ALU_input_updated_by_EX_ALU_input_imm_update] >>
+  `(s'.EX.EX_opc = (agp32 fext fbits (SUC t)).EX.EX_opc) /\
+  (s'.EX.EX_PC = (agp32 fext fbits (SUC t)).EX.EX_PC) /\
+  (s'.EX.EX_dataA = (agp32 fext fbits (SUC t)).EX.EX_dataA)`
+    by fs [agp32_same_EX_pipeline_items_after_EX_pipeline] >>
+  fs [EX_ALU_input_imm_update_def,ALU_input1_def,MUX_21_def] >>
+  METIS_TAC [agp32_Rel_ag32_EX_opc_correct,agp32_Rel_ag32_EX_dataA_correct,
+             agp32_Rel_ag32_EX_PC_correct]
+QED
+
+Theorem agp32_Rel_ag32_EX_ALU_input2_correct:
+  !fext fbits a t I.
+    is_sch_execute I (agp32 fext fbits) a ==>
+    is_sch_disable I (agp32 fext fbits) ==>
+    Rel I (fext t) (agp32 fext fbits (t-1)) (agp32 fext fbits t) a t ==>
+    I (3,SUC t) <> NONE ==>
+    (agp32 fext fbits (SUC t)).EX.EX_ALU_input2 = ALU_input2 (FUNPOW Next (THE (I (3,SUC t)) − 1) a)
+Proof
+  rw [] >> Q.ABBREV_TAC `s = agp32 fext fbits t` >>
+  Q.ABBREV_TAC `s' = procs [agp32_next_state;WB_pipeline;MEM_pipeline;EX_pipeline;
+                            REG_write;ID_pipeline;IF_PC_update;Acc_compute] (fext t) s s` >>
+  Q.ABBREV_TAC `s'' = procs [IF_instr_update;ID_opc_func_update;ID_imm_update;ID_data_update;
+                             ID_data_check_update;EX_ctrl_update] (fext (SUC t)) s' s'` >>
+  `(agp32 fext fbits (SUC t)).EX.EX_ALU_input2 =
+  (EX_ALU_input_imm_update (fext (SUC t)) s' s'').EX.EX_ALU_input2`
+    by fs [agp32_EX_ALU_input_updated_by_EX_ALU_input_imm_update] >>
+  `(s'.EX.EX_opc = (agp32 fext fbits (SUC t)).EX.EX_opc) /\
+  (s'.EX.EX_dataA = (agp32 fext fbits (SUC t)).EX.EX_dataA) /\
+  (s'.EX.EX_dataB = (agp32 fext fbits (SUC t)).EX.EX_dataB)`
+    by fs [agp32_same_EX_pipeline_items_after_EX_pipeline] >>
+  fs [EX_ALU_input_imm_update_def,ALU_input2_def,MUX_21_def] >>
+  METIS_TAC [agp32_Rel_ag32_EX_opc_correct,agp32_Rel_ag32_EX_dataA_correct,
+             agp32_Rel_ag32_EX_dataB_correct]
+QED
+
+(** EX_ALU_res **)
+Theorem agp32_Rel_ag32_EX_ALU_res_correct:
+  !fext fbits a t I.
+    is_sch I (agp32 fext fbits) a ==>
+    Rel I (fext t) (agp32 fext fbits (t-1)) (agp32 fext fbits t) a t ==>
+    I (3,SUC t) <> NONE ==>
+    (agp32 fext fbits (SUC t)).EX.EX_ALU_res = ALU_res (FUNPOW Next (THE (I (3,SUC t)) − 1) a)
+Proof
+  rw [] >> Q.ABBREV_TAC `s = agp32 fext fbits t` >>
+  Q.ABBREV_TAC `s' = procs [agp32_next_state;WB_pipeline;MEM_pipeline;EX_pipeline;
+                            REG_write;ID_pipeline;IF_PC_update;Acc_compute] (fext t) s s` >>
+  Q.ABBREV_TAC `s'' = procs [IF_instr_update;ID_opc_func_update;ID_imm_update;ID_data_update;
+                             ID_data_check_update;EX_ctrl_update;EX_ALU_input_imm_update] (fext (SUC t)) s' s'` >>
+  `(agp32 fext fbits (SUC t)).EX.EX_ALU_res = (EX_ALU_update (fext (SUC t)) s' s'').EX.EX_ALU_res`
+    by fs [agp32_EX_ALU_items_updated_by_EX_ALU_update] >>
+  `(s''.ID.ID_EX_write_enable = s.ID.ID_EX_write_enable) /\
+  (s''.EX.EX_overflow_flag = s.EX.EX_overflow_flag) /\
+  (s''.EX.EX_carry_flag = s.EX.EX_carry_flag) /\
+  (s''.EX.EX_ALU_res = s.EX.EX_ALU_res)` by cheat >>
+  `(s''.EX.EX_ALU_input1 = (agp32 fext fbits (SUC t)).EX.EX_ALU_input1) /\
+  (s''.EX.EX_ALU_input2 = (agp32 fext fbits (SUC t)).EX.EX_ALU_input2) /\
+  (s''.EX.EX_func = (agp32 fext fbits (SUC t)).EX.EX_func)` by cheat >>
+  Cases_on `enable_stg 3 (agp32 fext fbits t)` >-
+   (`s''.ID.ID_EX_write_enable` by fs [enable_stg_def,Abbr `s`] >>
+    `s''.EX.EX_func = func (FUNPOW Next (THE (I' (3,SUC t)) − 1) a)`
+      by fs [is_sch_def,agp32_Rel_ag32_EX_func_correct] >>
+    `s''.EX.EX_ALU_input1 = ALU_input1 (FUNPOW Next (THE (I' (3,SUC t)) − 1) a)`
+      by fs [is_sch_def,agp32_Rel_ag32_EX_ALU_input1_correct] >>
+    `s''.EX.EX_ALU_input2 = ALU_input2 (FUNPOW Next (THE (I' (3,SUC t)) − 1) a)`
+      by fs [is_sch_def,agp32_Rel_ag32_EX_ALU_input2_correct] >>
+    fs [EX_ALU_update_def,ALU_res_def,ALU_def] >>
+    Cases_on_word_value `(agp32 fext fbits (SUC t)).EX.EX_func` >> fs [] >-
+     (simp [word_mul_def,w2n_w2w] >> BBLAST_TAC) >-
+     (Cases_on `I' (3,t) <> NONE` >-
+       (fs [Rel_def] >>
+        `THE (I' (3,SUC t)) = THE (I' (3,t)) + 1`
+          by METIS_TAC [EX_instr_index_t_SUC_t_enable] >> fs []) >>
+      fs [] >> cheat) >-
+     (Cases_on `I' (3,t) <> NONE` >-
+       (fs [Rel_def] >>
+        `THE (I' (3,SUC t)) = THE (I' (3,t)) + 1`
+          by METIS_TAC [EX_instr_index_t_SUC_t_enable] >> fs []) >>
+      fs [] >> cheat) >-
+     (`s.EX.EX_carry_flag = (FUNPOW Next (THE (I' (3,SUC t)) − 1) a).CarryFlag` by cheat >>
+      rw [ALU_correct_v2w_carry33_lem,ALU_correct_v2w_carry32_lem] >>
+      BBLAST_TAC) >>
+    BBLAST_TAC) >>
+  `I' (3,SUC t) = I' (3,t)` by fs [is_sch_def,is_sch_disable_def] >>
+  `~s''.ID.ID_EX_write_enable` by fs [enable_stg_def,Abbr `s`] >>
+  rw [EX_ALU_update_def] >>
+  fs [Rel_def,EX_Rel_def]
+QED
+
 
 (* EX stage *)
 Theorem agp32_Rel_ag32_EX_Rel_correct:
@@ -660,7 +823,9 @@ Proof
       agp32_Rel_ag32_EX_imm_correct,agp32_Rel_ag32_EX_opc_correct,
       agp32_Rel_ag32_EX_func_correct,agp32_Rel_ag32_EX_write_reg_correct,
       agp32_Rel_ag32_EX_dataA_correct,agp32_Rel_ag32_EX_dataB_correct,
-      agp32_Rel_ag32_EX_dataW_correct] >>
+      agp32_Rel_ag32_EX_dataW_correct,agp32_Rel_ag32_EX_imm_updated_correct_not_LoadUpperConstant,
+      agp32_Rel_ag32_EX_imm_updated_correct_LoadUpperConstant,
+      agp32_Rel_ag32_EX_ALU_input1_correct,agp32_Rel_ag32_EX_ALU_input2_correct] >>
   cheat
 QED
 
